examples/wysteria/sem.fst
@@ -1,9 +1,12 @@
 (*--build-config
     options:--admit_fsi FStar.OrdSet --admit_fsi FStar.OrdMap --admit_fsi Prins --admit_fsi FFI;
-    other-files:ordset.fsi ordmap.fsi classical.fst prins.fsi ast.fst ffi.fsi
+    other-files:ghost.fst listTot.fst ordset.fsi ordmap.fsi classical.fst prins.fsi ast.fst ffi.fsi
  --*)
 
 module Semantics
+
+open FStar.Ghost
+open FStar.List.Tot
 
 open FStar.OrdMap
 open FStar.OrdSet
@@ -52,7 +55,7 @@ let is_Some x = match x with
 
 (* TODO: FIXME: workaround for projectors *)
 val en_of_conf: config -> Tot env
-let en_of_conf (Conf _ _ _ en _) = en
+let en_of_conf (Conf _ _ _ en _ _) = en
 
 let pre_evar (c:config) =
   is_T_exp (t_of_conf c) && is_E_var (e_of_exp (e_of_t_exp (t_of_conf c))) &&
@@ -83,121 +86,154 @@ let pre_ematch (c:config) =
 type comp = | Do | Skip | NA
 
 val step_aspar_e1: c:config{pre_easpar c} -> Tot config
-let step_aspar_e1 (Conf l m s en (T_exp (Exp (E_aspar e1 e2) _))) =
-  Conf l m ((Frame m en (F_aspar_ps e2))::s) en (T_exp e1)
+let step_aspar_e1 (Conf l m s en (T_exp (Exp (E_aspar e1 e2) _)) tr) =
+  Conf l m ((Frame m en (F_aspar_ps e2) tr)::s) en (T_exp e1) (hide [])
   
 val step_box_e1: c:config{pre_ebox c} -> Tot config
-let step_box_e1 (Conf l m s en (T_exp (Exp (E_box e1 e2) _))) =
-  Conf l m ((Frame m en (F_box_ps e2))::s) en (T_exp e1)
+let step_box_e1 (Conf l m s en (T_exp (Exp (E_box e1 e2) _)) tr) =
+  Conf l m ((Frame m en (F_box_ps e2) tr)::s) en (T_exp e1) (hide [])
 
 val step_unbox_e: c:config{pre_eunbox c} -> Tot config
-let step_unbox_e (Conf l m s en (T_exp (Exp (E_unbox e) _))) =
-  Conf l m ((Frame m en F_unbox)::s) en (T_exp e)
+let step_unbox_e (Conf l m s en (T_exp (Exp (E_unbox e) _)) tr) =
+  Conf l m ((Frame m en F_unbox tr)::s) en (T_exp e) (hide [])
  
 val step_mkwire_e1: c:config{pre_emkwire c} -> Tot config
-let step_mkwire_e1 (Conf l m s en (T_exp (Exp (E_mkwire e1 e2) _))) =
-  Conf l m ((Frame m en (F_mkwire_ps e2))::s) en (T_exp e1)
+let step_mkwire_e1 (Conf l m s en (T_exp (Exp (E_mkwire e1 e2) _)) tr) =
+  Conf l m ((Frame m en (F_mkwire_ps e2) tr)::s) en (T_exp e1) (hide [])
 
 val step_projwire_e1: c:config{pre_eprojwire c} -> Tot config
-let step_projwire_e1 (Conf l m s en (T_exp (Exp (E_projwire e1 e2) _))) =
-  Conf l m ((Frame m en (F_projwire_p e2))::s) en (T_exp e1)
+let step_projwire_e1 (Conf l m s en (T_exp (Exp (E_projwire e1 e2) _)) tr) =
+  Conf l m ((Frame m en (F_projwire_p e2) tr)::s) en (T_exp e1) (hide [])
 
 val step_concatwire_e1: c:config{pre_econcatwire c} -> Tot config
-let step_concatwire_e1 (Conf l m s en (T_exp (Exp (E_concatwire e1 e2) _))) =
-  Conf l m ((Frame m en (F_concatwire_e1 e2))::s) en (T_exp e1)
+let step_concatwire_e1 (Conf l m s en (T_exp (Exp (E_concatwire e1 e2) _)) tr) =
+  Conf l m ((Frame m en (F_concatwire_e1 e2) tr)::s) en (T_exp e1) (hide [])
 
 val step_const: c:config{pre_econst c} -> Tot config
-let step_const (Conf l m s en (T_exp (Exp (E_const c) _))) =
-  Conf l m s en (T_val (V_const c))
+let step_const (Conf l m s en (T_exp (Exp (E_const c) _)) tr) =
+  Conf l m s en (T_val (V_const c)) tr
 
 val step_var: c:config{pre_evar c} -> Tot config
-let step_var (Conf l m s en (T_exp (Exp (E_var x) _))) =
+let step_var (Conf l m s en (T_exp (Exp (E_var x) _)) tr) =
   let Some (D_v _ v) = en x in
-  Conf l m s en (T_val v)
+  Conf l m s en (T_val v) tr
 
 val step_let_e1: c:config{pre_elet c} -> Tot config
-let step_let_e1 (Conf l m s en (T_exp (Exp (E_let x e1 e2) _))) =
-  Conf l m ((Frame m en (F_let x e2))::s) en (T_exp e1)
+let step_let_e1 (Conf l m s en (T_exp (Exp (E_let x e1 e2) _)) tr) =
+  Conf l m ((Frame m en (F_let x e2) tr)::s) en (T_exp e1) (hide [])
 
 val step_abs: c:config{pre_eabs c} -> Tot config
-let step_abs (Conf l m s en (T_exp (Exp (E_abs x e) _))) =
-  Conf l m s en (T_val (V_clos en x e))
+let step_abs (Conf l m s en (T_exp (Exp (E_abs x e) _)) tr) =
+  Conf l m s en (T_val (V_clos en x e)) tr
  
 val step_fix: c:config{pre_efix c} -> Tot config
-let step_fix (Conf l m s en (T_exp (Exp (E_fix f x e) _))) =
-  Conf l m s en (T_val (V_fix_clos en f x e))
+let step_fix (Conf l m s en (T_exp (Exp (E_fix f x e) _)) tr) =
+  Conf l m s en (T_val (V_fix_clos en f x e)) tr
 
 val step_empabs: c:config{pre_eempabs c} -> Tot config
-let step_empabs (Conf l m s en (T_exp (Exp (E_empabs x e) _))) =
-  Conf l m s en (T_val (V_emp_clos x e))
+let step_empabs (Conf l m s en (T_exp (Exp (E_empabs x e) _)) tr) =
+  Conf l m s en (T_val (V_emp_clos x e)) tr
 
 val step_app_e1: c:config{pre_eapp c} -> Tot config
-let step_app_e1 (Conf l m s en (T_exp (Exp (E_app e1 e2) _))) =
-  Conf l m ((Frame m en (F_app_e1 e2))::s) en (T_exp e1)
+let step_app_e1 (Conf l m s en (T_exp (Exp (E_app e1 e2) _)) tr) =
+  Conf l m ((Frame m en (F_app_e1 e2) tr)::s) en (T_exp e1) (hide [])
  
 val step_ffi_e: c:config{pre_effi c} -> Tot config
-let step_ffi_e (Conf l m s en (T_exp (Exp (E_ffi fn es) _))) = match es with
-  | []    -> Conf l m s en (T_red (R_ffi fn []))
-  | e::tl -> Conf l m ((Frame m en (F_ffi fn tl []))::s) en (T_exp e)
+let step_ffi_e (Conf l m s en (T_exp (Exp (E_ffi fn es) _)) tr) = match es with
+  | []    -> Conf l m s en (T_red (R_ffi fn [])) tr
+  | e::tl  -> Conf l m ((Frame m en (F_ffi fn tl []) tr)::s) en (T_exp e) (hide [])
   
 val step_match_e: c:config{pre_ematch c} -> Tot config
-let step_match_e (Conf l m s en (T_exp (Exp (E_match e pats) _))) =
-  Conf l m ((Frame m en (F_match pats))::s) en (T_exp e)
+let step_match_e (Conf l m s en (T_exp (Exp (E_match e pats) _)) tr) =
+  Conf l m ((Frame m en (F_match pats) tr)::s) en (T_exp e) (hide [])
+
+val concat_traces: erased trace -> erased trace -> Tot (erased trace)
+let concat_traces t1 t2 = elift2 append t1 t2
+
+(* val append_flat_lemma: t1:trace -> t2:trace *)
+(*                        -> Lemma (requires (is_flat_trace t1 /\ is_flat_trace t2)) *)
+(* 		               (ensures (is_flat_trace (append t1 t2))) *)
+(* 		         [SMTPat (is_flat_trace (append t1 t2))] *)
+(* let rec append_flat_lemma t1 t2 = match t1 with *)
+(*   | []   -> () *)
+(*   | _::tl -> append_flat_lemma tl t2 *)
 
 val step_aspar_e2: c:config{is_value_ps c /\ is_sframe c is_F_aspar_ps}
                   -> Tot config
-let step_aspar_e2 (Conf l _ ((Frame m en (F_aspar_ps e))::s) _
-                       (T_val (V_const (C_prins ps)))) =
-  Conf l m ((Frame m en (F_aspar_e ps))::s) en (T_exp e)
+let step_aspar_e2 (Conf l _ ((Frame m en (F_aspar_ps e) tr)::s) _
+                       (T_val (V_const (C_prins ps))) tr') =
+  Conf l m ((Frame m en (F_aspar_e ps) (concat_traces tr tr'))::s) en (T_exp e) (hide [])
+
+val vals_traces_h_append_lemma:
+  tr1:trace{vals_trace_h tr1} -> tr2:trace{vals_trace_h tr2}
+  -> Lemma (requires (True)) (ensures (vals_trace_h (append tr1 tr2)))
+let rec vals_traces_h_append_lemma tr1 tr2 = match tr1 with
+  | []   -> ()
+  | _::tl -> vals_traces_h_append_lemma tl tr2
+
+assume val vals_traces_h_append_lemma_forall:
+  unit -> Lemma (requires (True)) (ensures (forall tr1 tr2. vals_trace_h tr1 ==>
+                                                   vals_trace_h tr2 ==>
+						   vals_trace_h (append tr1 tr2)))
+
+val vals_traces_concat_lemma:
+  tr1:erased trace{vals_trace tr1}
+  -> tr2:erased trace{vals_trace tr2}
+  -> Lemma (requires (True)) (ensures (vals_trace (concat_traces tr1 tr2)))
+    [SMTPat (vals_trace (concat_traces tr1 tr2))]
+let vals_traces_concat_lemma tr1 tr2 =
+  vals_traces_h_append_lemma_forall ();
+  let _ = assert (vals_trace_h (append (reveal tr1) (reveal tr2))) in
+  ()
 
 val step_box_e2: c:config{is_value_ps c /\ is_sframe c is_F_box_ps}
                   -> Tot config
-let step_box_e2 (Conf l _ ((Frame m en (F_box_ps e))::s) _
-                      (T_val (V_const (C_prins ps)))) =
-  Conf l m ((Frame m en (F_box_e ps))::s) en (T_exp e)
+let step_box_e2 (Conf l _ ((Frame m en (F_box_ps e) tr)::s) _
+                      (T_val (V_const (C_prins ps))) tr') =
+  Conf l m ((Frame m en (F_box_e ps) (concat_traces tr tr'))::s) en (T_exp e) (hide [])
 
 val step_mkwire_e2: c:config{is_value c /\ is_sframe c is_F_mkwire_ps}
                    -> Tot config
-let step_mkwire_e2 (Conf l _ ((Frame m en (F_mkwire_ps e))::s) _
-                        (T_val v)) =
-  Conf l m ((Frame m en (F_mkwire_e v))::s) en (T_exp e)
+let step_mkwire_e2 (Conf l _ ((Frame m en (F_mkwire_ps e) tr)::s) _
+                        (T_val v) tr') =
+  Conf l m ((Frame m en (F_mkwire_e v) (concat_traces tr tr'))::s) en (T_exp e) (hide [])
 
 val step_projwire_e2: c:config{is_value_p c /\ is_sframe c is_F_projwire_p}
                      -> Tot config
-let step_projwire_e2 (Conf l _ ((Frame m en (F_projwire_p e))::s) _
-                          (T_val (V_const (C_prin p)))) =
-  Conf l m ((Frame m en (F_projwire_e p))::s) en (T_exp e)
+let step_projwire_e2 (Conf l _ ((Frame m en (F_projwire_p e) tr)::s) _
+                          (T_val (V_const (C_prin p))) tr') =
+  Conf l m ((Frame m en (F_projwire_e p) (concat_traces tr tr'))::s) en (T_exp e) (hide [])
 
 val step_concatwire_e2: c:config{is_value c /\ is_sframe c is_F_concatwire_e1}
                        -> Tot config
-let step_concatwire_e2 (Conf l _ ((Frame m en (F_concatwire_e1 e))::s) _
-                            (T_val v)) =
-  Conf l m ((Frame m en (F_concatwire_e2 v))::s) en (T_exp e)
+let step_concatwire_e2 (Conf l _ ((Frame m en (F_concatwire_e1 e) tr)::s) _
+                            (T_val v) tr') =
+  Conf l m ((Frame m en (F_concatwire_e2 v) (concat_traces tr tr'))::s) en (T_exp e) (hide [])
 
 val step_app_e2: c:config{is_value c /\ is_sframe c is_F_app_e1}
                 -> Tot config
-let step_app_e2 (Conf l _ ((Frame m en (F_app_e1 e2))::s) _ (T_val v)) =
-  Conf l m ((Frame m en (F_app_e2 v))::s) en (T_exp e2)
+let step_app_e2 (Conf l _ ((Frame m en (F_app_e1 e2) tr)::s) _ (T_val v) tr') =
+  Conf l m ((Frame m en (F_app_e2 v) (concat_traces tr tr'))::s) en (T_exp e2) (hide [])
 
 val step_ffi_l: c:config{is_value c /\ is_sframe c is_F_ffi} -> Tot config
-let step_ffi_l (Conf l _ ((Frame m en (F_ffi fn es vs))::s) _ (T_val #meta v)) =
+let step_ffi_l (Conf l _ ((Frame m en (F_ffi fn es vs) tr)::s) _ (T_val #meta v) tr') =
   match es with
-    | []    -> Conf l m s en (T_red (R_ffi fn ((D_v meta v)::vs)))
-    | e::tl -> Conf l m ((Frame m en (F_ffi fn tl ((D_v meta v)::vs)))::s) en (T_exp e)
+    | []    -> Conf l m s en (T_red (R_ffi fn ((D_v meta v)::vs))) (concat_traces tr tr')
+    | e::tl -> Conf l m ((Frame m en (F_ffi fn tl ((D_v meta v)::vs)) (concat_traces tr tr'))::s) en (T_exp e) (hide [])
     
 val step_match_red: c:config{is_value c /\ is_sframe c is_F_match} -> Tot config
-let step_match_red (Conf l _ ((Frame m en (F_match pats))::s) _ (T_val v)) =
-  Conf l m s en (T_red (R_match v pats))
+let step_match_red (Conf l _ ((Frame m en (F_match pats) tr)::s) _ (T_val v) tr') =
+  Conf l m s en (T_red (R_match v pats)) (concat_traces tr tr')
   
 val step_aspar_red: c:config{is_value c /\ is_sframe c is_F_aspar_e}
                    -> Tot config
-let step_aspar_red (Conf l _ ((Frame m en (F_aspar_e ps))::s) _ (T_val v)) =
-  Conf l m s en (T_red (R_aspar ps v))
+let step_aspar_red (Conf l _ ((Frame m en (F_aspar_e ps) tr)::s) _ (T_val v) tr') =
+  Conf l m s en (T_red (R_aspar ps v)) (concat_traces tr tr')
 
 val step_box_red: c:config{is_value c /\ is_sframe c is_F_box_e}
                    -> Tot config
-let step_box_red (Conf l _ ((Frame m en (F_box_e ps))::s) _ (T_val v)) =
-  Conf l m s en (T_red (R_box ps v))
+let step_box_red (Conf l _ ((Frame m en (F_box_e ps) tr)::s) _ (T_val v) tr') =
+  Conf l m s en (T_red (R_box ps v)) (concat_traces tr tr')
 
 (*val step_box_red: c:config{is_value c /\ is_sframe c is_F_box_e}
                  -> Tot config
@@ -206,37 +242,37 @@ let step_box_red (Conf l _ ((Frame m en (F_box_e ps))::s) _ (T_val v)) =
 
 val step_unbox_red: c:config{is_value c /\ is_sframe c is_F_unbox}
                    -> Tot config
-let step_unbox_red (Conf l _ ((Frame m en F_unbox)::s) _ (T_val v)) =
-  Conf l m s en (T_red (R_unbox v))
+let step_unbox_red (Conf l _ ((Frame m en F_unbox tr)::s) _ (T_val v) tr') =
+  Conf l m s en (T_red (R_unbox v)) (concat_traces tr tr')
 
 val step_projwire_red: c:config{is_value c /\ is_sframe c is_F_projwire_e}
                       -> Tot config
-let step_projwire_red (Conf l _ ((Frame m en (F_projwire_e p))::s) _ (T_val v)) =
-  Conf l m s en (T_red (R_projwire p v))
+let step_projwire_red (Conf l _ ((Frame m en (F_projwire_e p) tr)::s) _ (T_val v) tr') =
+  Conf l m s en (T_red (R_projwire p v)) (concat_traces tr tr')
 
 val step_mkwire_red: c:config{is_value c /\ is_sframe c is_F_mkwire_e}
                     -> Tot config
-let step_mkwire_red (Conf l _ ((Frame m en (F_mkwire_e v1))::s) _ (T_val v2)) =
-  Conf l m s en (T_red (R_mkwire v1 v2))
+let step_mkwire_red (Conf l _ ((Frame m en (F_mkwire_e v1) tr)::s) _ (T_val v2) tr') =
+  Conf l m s en (T_red (R_mkwire v1 v2)) (concat_traces tr tr')
 
 val step_concatwire_red: c:config{is_value c /\ is_sframe c is_F_concatwire_e2}
                         -> Tot config
-let step_concatwire_red (Conf l _ ((Frame m en (F_concatwire_e2 v1))::s) _ (T_val v2)) =
-  Conf l m s en (T_red (R_concatwire v1 v2))
+let step_concatwire_red (Conf l _ ((Frame m en (F_concatwire_e2 v1) tr)::s) _ (T_val v2) tr') =
+  Conf l m s en (T_red (R_concatwire v1 v2)) (concat_traces tr tr')
 
 val step_let_red: c:config{is_value c /\ is_sframe c is_F_let}
                  -> Tot config
-let step_let_red (Conf l _ ((Frame m en (F_let x e2))::s) _ (T_val v)) =
-  Conf l m s en (T_red (R_let x v e2))
+let step_let_red (Conf l _ ((Frame m en (F_let x e2) tr)::s) _ (T_val v) tr') =
+  Conf l m s en (T_red (R_let x v e2)) (concat_traces tr tr')
 
 val step_app_red: c:config{is_value c /\ is_sframe c is_F_app_e2}
                  -> Tot config
-let step_app_red (Conf l _ ((Frame m en (F_app_e2 v1))::s) _ (T_val v2)) =
-  Conf l m s en (T_red (R_app v1 v2))
+let step_app_red (Conf l _ ((Frame m en (F_app_e2 v1) tr)::s) _ (T_val v2) tr') =
+  Conf l m s en (T_red (R_app v1 v2)) (concat_traces tr tr')
 
 val pre_aspar: config -> Tot comp
 let pre_aspar c = match c with
-  | Conf l (Mode Par ps1) _ _ (T_red (R_aspar ps2 v)) ->
+  | Conf l (Mode Par ps1) _ _ (T_red (R_aspar ps2 v)) _ ->
     if is_clos v then
       if src l then
         if subset ps2 ps1 then Do else NA
@@ -248,10 +284,10 @@ let pre_aspar c = match c with
 
 val step_aspar: c:config{not (pre_aspar c = NA)} -> Tot config
 let step_aspar c = match c with
-  | Conf l m s en' (T_red (R_aspar ps v)) ->
+  | Conf l m s en' (T_red (R_aspar ps v)) tr ->
     let en, x, e = get_en_b v in
     let m'  = if src l then Mode Par ps else m in
-    let s'  = (Frame m en' (F_aspar_ret ps))::s in
+    let s'  = (Frame m en' (F_aspar_ret ps) tr)::s in
 
     (*
      * for parties not in ps, the choice of empty_env is arbitrary
@@ -265,11 +301,11 @@ let step_aspar c = match c with
         else empty_env, T_val V_emp
     in
 
-    Conf l m' s' en' t'
+    Conf l m' s' en' t' (hide [])
 
 val pre_box: c:config -> Tot comp
 let pre_box c = match c with
-  | Conf l (Mode _ ps) _ _ (T_red (R_box #meta ps' v)) ->
+  | Conf l (Mode _ ps) _ _ (T_red (R_box #meta ps' v)) _ ->
     if is_meta_boxable ps' meta then
       if src l then
         if subset ps' ps then Do else NA
@@ -279,17 +315,17 @@ let pre_box c = match c with
   | _ -> NA
 
 val step_box: c:config{pre_box c = Do} -> Tot config
-let step_box (Conf l m s en (T_red (R_box ps' v))) =
+let step_box (Conf l m s en (T_red (R_box ps' v)) tr) =
   let Mode as_m ps = m in
   if src l || as_m = Sec then
-    Conf l m s en (T_val (V_box ps' v))
+    Conf l m s en (T_val (V_box ps' v)) tr
   else
-    if subset ps ps' then Conf l m s en (T_val (V_box ps' v))
-    else Conf l m s en (T_val (V_box ps' V_emp))
+    if subset ps ps' then Conf l m s en (T_val (V_box ps' v)) tr
+    else Conf l m s en (T_val (V_box ps' V_emp)) tr // TODO: FIXME: V_emp or v ?
 
 val pre_unbox: config -> Tot comp
 let pre_unbox c = match c with
-  | Conf _ (Mode as_m ps1) _ _ (T_red (R_unbox (V_box ps2 _))) ->
+  | Conf _ (Mode as_m ps1) _ _ (T_red (R_unbox (V_box ps2 _))) _ ->
     if as_m = Par then
       if subset ps1 ps2 then Do else NA
     else
@@ -299,19 +335,19 @@ let pre_unbox c = match c with
 
 val step_unbox: c:config{pre_unbox c = Do} -> Tot config
 let step_unbox c = match c with
-  | Conf l m s en (T_red (R_unbox (V_box _ v))) -> Conf l m s en (T_val v)
+  | Conf l m s en (T_red (R_unbox (V_box _ v))) tr -> Conf l m s en (T_val v) tr
 
 val pre_mkwire: config -> Tot comp
 let pre_mkwire c = match c with
   | Conf l (Mode Par ps) _ _ (T_red (R_mkwire (V_const (C_prins ps'))
-                                                       (V_box #mv ps'' _))) ->
+                                                       (V_box #mv ps'' _))) _ ->
     if is_meta_wireable mv then
       if src l then
         if subset ps' ps && subset ps' ps'' then Do else NA
       else Do
     else NA
  
-  | Conf l (Mode Sec ps) _ _ (T_red (R_mkwire #mps #mv (V_const (C_prins ps')) _)) ->
+  | Conf l (Mode Sec ps) _ _ (T_red (R_mkwire #mps #mv (V_const (C_prins ps')) _)) _ ->
     if is_meta_wireable mv then
       if subset ps' ps then Do else NA
     else NA
@@ -326,7 +362,7 @@ let mconst_on eps v = const_on eps v
 val step_mkwire: c:config{pre_mkwire c = Do} -> Tot config
 let step_mkwire c = match c with
   | Conf l (Mode Par ps) s en (T_red (R_mkwire (V_const (C_prins ps'))
-                                                       (V_box _ v))) ->
+                                                       (V_box _ v))) tr ->
     let eps, w =
       if src l then ps', mconst_on ps' v
       else
@@ -334,14 +370,14 @@ let step_mkwire c = match c with
           ps, mconst_on ps v
         else empty, OrdMap.empty
     in
-    Conf l (Mode Par ps) s en (T_val (V_wire eps w))
+    Conf l (Mode Par ps) s en (T_val (V_wire eps w)) tr
 
-  | Conf l (Mode Sec ps) s en (T_red (R_mkwire (V_const (C_prins ps')) v)) ->
-    Conf l (Mode Sec ps) s en (T_val (V_wire ps' (mconst_on ps' v)))
+  | Conf l (Mode Sec ps) s en (T_red (R_mkwire (V_const (C_prins ps')) v)) tr ->
+    Conf l (Mode Sec ps) s en (T_val (V_wire ps' (mconst_on ps' v))) tr
 
 val pre_projwire: config -> Tot comp
 let pre_projwire c = match c with
-  | Conf _ (Mode as_m ps) _ _ (T_red (R_projwire p (V_wire eps _))) ->
+  | Conf _ (Mode as_m ps) _ _ (T_red (R_projwire p (V_wire eps _))) _ ->
     if as_m = Par then
       if ps = singleton p && mem p eps then Do else NA
     else
@@ -355,12 +391,12 @@ let v_of_some (Some x) = x
 
 val step_projwire: c:config{pre_projwire c = Do} -> Tot config
 let step_projwire c = match c with
-  | Conf l m s en (T_red (R_projwire p (V_wire _ w))) ->
-    Conf l m s en (T_val (v_of_some (select p w)))
+  | Conf l m s en (T_red (R_projwire p (V_wire _ w))) tr ->
+    Conf l m s en (T_val (v_of_some (select p w))) tr
 
 val pre_concatwire: config -> Tot comp
 let pre_concatwire c = match c with
-  | Conf _ _ _ _ (T_red (R_concatwire (V_wire eps1 _) (V_wire eps2 _))) ->
+  | Conf _ _ _ _ (T_red (R_concatwire (V_wire eps1 _) (V_wire eps2 _))) tr ->
     if intersect eps1 eps2 = empty then Do else NA
    
   | _ -> NA
@@ -401,30 +437,30 @@ let rec compose_wires #eps1 #eps2 w1 w2 eps =
 
 val step_concatwire: c:config{pre_concatwire c = Do} -> Tot config
 let step_concatwire c = match c with
-  | Conf l m s en (T_red (R_concatwire (V_wire eps1 w1) (V_wire eps2 w2))) ->
-    Conf l m s en (T_val (V_wire (union eps1 eps2) (compose_wires #eps1 #eps2 w1 w2 eps1)))
+  | Conf l m s en (T_red (R_concatwire (V_wire eps1 w1) (V_wire eps2 w2))) tr ->
+    Conf l m s en (T_val (V_wire (union eps1 eps2) (compose_wires #eps1 #eps2 w1 w2 eps1))) tr
 
 val is_let_redex: c:config -> Tot bool
 let is_let_redex c = match c with
-  | Conf _ _ _ _ (T_red (R_let _ _ _)) -> true
-  | _                                  -> false
+  | Conf _ _ _ _ (T_red (R_let _ _ _)) _ -> true
+  | _                                    -> false
 
 val step_let: c:config{is_let_redex c} -> Tot config
 let step_let c = match c with
-  | Conf l m s en (T_red (R_let x v1 e2)) ->
-    Conf l m s (update_env en x v1) (T_exp e2)
+  | Conf l m s en (T_red (R_let x v1 e2)) tr ->
+    Conf l m s (update_env en x v1) (T_exp e2) tr
 
 val is_app_redex: c:config -> Tot bool
 let is_app_redex c = match c with
-  | Conf _ _ _ _ (T_red (R_app v _)) -> is_clos v
+  | Conf _ _ _ _ (T_red (R_app v _)) _ -> is_clos v
 
   | _ -> false
 
 val step_app: c:config{is_app_redex c} -> Tot config
 let step_app c = match c with
-  | Conf l m s _ (T_red (R_app f v)) ->
+  | Conf l m s _ (T_red (R_app f v)) tr ->
     let (en, x, e) = get_en_b f in
-    Conf l m s (update_env en x v) (T_exp e)
+    Conf l m s (update_env en x v) (T_exp e) tr
 
 val is_valid_ffi_v: #meta:v_meta -> v:value meta -> Tot bool
 let is_valid_ffi_v #meta v = match v with
@@ -443,19 +479,19 @@ let rec is_valid_ffi_vs vs = match vs with
 
 val pre_ffi: config -> Tot comp
 let pre_ffi c = match c with
-  | Conf _ _ _ _ (T_red (R_ffi _ vs)) -> Do
+  | Conf _ _ _ _ (T_red (R_ffi _ vs)) _ -> Do
     (*if is_valid_ffi_vs vs then Do else NA*)
   
   | _ -> NA
 
 val step_ffi: c:config{pre_ffi c = Do} -> Tot config
-let step_ffi (Conf l m s en (T_red (R_ffi fn vs))) =
+let step_ffi (Conf l m s en (T_red (R_ffi fn vs)) tr) =
   let D_v _ v = FFI.exec_ffi fn vs in
-  Conf l m s en (T_val v)
+  Conf l m s en (T_val v) tr
 
 val pre_match: config -> Tot comp
 let pre_match c = match c with
-  | Conf _ _ _ _ (T_red (R_match _ _)) -> Do
+  | Conf _ _ _ _ (T_red (R_match _ _)) _ -> Do
   
   | _ -> NA
 
@@ -476,12 +512,12 @@ let rec get_next_exp #meta pats v = match pats with
     if match_pat p v then e else get_next_exp #meta tl v
 
 val step_match: c:config{pre_match c = Do} -> Tot config
-let step_match (Conf l m s en (T_red (R_match v pats))) =
-  Conf l m s en (T_exp (get_next_exp pats v))
+let step_match (Conf l m s en (T_red (R_match v pats)) tr) =
+  Conf l m s en (T_exp (get_next_exp pats v)) tr
 
 val pre_aspar_ret: config -> Tot comp
 let pre_aspar_ret c = match c with
-  | Conf _ _ ((Frame _ _ (F_aspar_ret ps))::_) _ (T_val #meta _) ->
+  | Conf _ _ ((Frame _ _ (F_aspar_ret ps) _)::_) _ (T_val #meta _) _ ->
     if is_meta_boxable ps meta then Do else NA
       (*if src l then
         if subset ps2 ps1 then Do else NA
@@ -490,32 +526,41 @@ let pre_aspar_ret c = match c with
 *)
   | _ -> NA
 
+val scope_trace: prins -> trace -> Tot trace
+let scope_trace ps t = [ Tr_scope ps t ]
+
 val step_aspar_ret: c:config{pre_aspar_ret c = Do} -> Tot config
 let step_aspar_ret c = match c with
-  | Conf l _ ((Frame m en (F_aspar_ret ps))::s) _ (T_val v)
-    -> Conf l m s en (T_val (V_box ps v))
+  | Conf l _ ((Frame m en (F_aspar_ret ps) tr)::s) _ (T_val v) tr' ->
+    let tr =
+      if l = Source then
+	concat_traces tr (elift1 (scope_trace ps) tr')
+      else concat_traces tr tr'
+    in
+	
+    Conf l m s en (T_val (V_box ps v)) tr
 
 let pre_eassec (c:config) =
   is_T_exp (t_of_conf c) && is_E_assec (e_of_exp (e_of_t_exp (t_of_conf c)))
 
 val step_assec_e1: c:config{pre_eassec c} -> Tot config
-let step_assec_e1 (Conf l m s en (T_exp (Exp (E_assec e1 e2) _))) =
-  Conf l m ((Frame m en (F_assec_ps e2))::s) en (T_exp e1)
+let step_assec_e1 (Conf l m s en (T_exp (Exp (E_assec e1 e2) _)) tr) =
+  Conf l m ((Frame m en (F_assec_ps e2) tr)::s) en (T_exp e1) (hide [])
 
 val step_assec_e2: c:config{is_value_ps c /\ is_sframe c is_F_assec_ps}
                   -> Tot config
-let step_assec_e2 (Conf l _ ((Frame m en (F_assec_ps e))::s) _
-                       (T_val (V_const (C_prins ps)))) =
-  Conf l m ((Frame m en (F_assec_e ps))::s) en (T_exp e)
+let step_assec_e2 (Conf l _ ((Frame m en (F_assec_ps e) tr)::s) _
+                       (T_val (V_const (C_prins ps))) tr') =
+  Conf l m ((Frame m en (F_assec_e ps) (concat_traces tr tr'))::s) en (T_exp e) (hide [])
 
 val step_assec_red: c:config{is_value c /\ is_sframe c is_F_assec_e}
                    -> Tot config
-let step_assec_red (Conf l _ ((Frame m en (F_assec_e ps))::s) _ (T_val v)) =
-  Conf l m s en (T_red (R_assec ps v))
+let step_assec_red (Conf l _ ((Frame m en (F_assec_e ps) tr)::s) _ (T_val v) tr') =
+  Conf l m s en (T_red (R_assec ps v)) (concat_traces tr tr')
 
 val pre_assec: config -> Tot comp
 let pre_assec c = match c with
-  | Conf l (Mode as_m ps1) _ _ (T_red (R_assec ps2 v)) ->
+  | Conf l (Mode as_m ps1) _ _ (T_red (R_assec ps2 v)) _ ->
     if is_clos v then
       if l = Source || as_m = Sec then
         if ps1 = ps2 then Do else NA
@@ -526,14 +571,19 @@ let pre_assec c = match c with
 
 val step_assec: c:config{not (pre_assec c = NA)} -> Tot config
 let step_assec c = match c with
-  | Conf l m s en' (T_red (R_assec ps v)) ->
+  | Conf l m s en' (T_red (R_assec ps v)) tr ->
     let (en, x, e) = get_en_b v in
-    Conf l (Mode Sec ps) ((Frame m en' F_assec_ret)::s)
-           (update_env en x (V_const C_unit)) (T_exp e)
+    Conf l (Mode Sec ps) ((Frame m en' F_assec_ret tr)::s)
+           (update_env en x (V_const C_unit)) (T_exp e) (hide [])
 
 val step_assec_ret: c:config{is_value c /\ is_sframe c is_F_assec_ret}
                    -> Tot config
-let step_assec_ret (Conf l _ ((Frame m en F_assec_ret)::s) _ t) = Conf l m s en t
+let step_assec_ret (Conf l _ ((Frame m en F_assec_ret tr)::s) _ t tr') =
+  let tr' =
+    if m_of_mode m = Par then concat_traces tr (hide [ Tr_val (T_val.v t) ])
+    else tr
+  in
+  Conf l m s en t tr'
 
 type sstep: config -> config -> Type =
   | C_aspar_ps:
