examples/wysteria/theory.fst
@@ -1,9 +1,12 @@
 (*--build-config
     options:--admit_fsi FStar.Set --admit_fsi FStar.OrdSet --admit_fsi FStar.OrdMap --admit_fsi Prins --admit_fsi FFI --z3timeout 10 --__temp_no_proj;
-    other-files:set.fsi ordset.fsi ordmap.fsi constr.fst ext.fst classical.fst prins.fsi ast.fst ffi.fsi sem.fst
+    other-files:ghost.fst listTot.fst set.fsi ordset.fsi ordmap.fsi constr.fst ext.fst classical.fst prins.fsi ast.fst ffi.fsi sem.fst
  --*)
 
 module Metatheory
+
+open FStar.Ghost
+open FStar.List.Tot
 
 open FStar.OrdMap
 open FStar.OrdSet
@@ -119,11 +122,43 @@ let slice_f'_sps ps f = match f with
   | F_ffi fn es vs    -> F_ffi fn es (slice_vs_sps ps vs)
   | F_match      _    -> f
 
+val slice_tr_sps_h: prins -> tr:trace -> Tot trace
+let rec slice_tr_sps_h ps tr = match tr with
+  | []            -> []
+  | (Tr_val v)::tl -> Tr_val (D_v.v (slice_v_sps ps v))::slice_tr_sps_h ps tl
+  | _::tl          -> slice_tr_sps_h ps tl // this case never arises
+
+val slice_tr_sps_h_vals_lemma:
+  ps:prins -> tr:trace
+  -> Lemma (requires (True))
+          (ensures (vals_trace_h (slice_tr_sps_h ps tr)))
+let rec slice_tr_sps_h_vals_lemma ps tr = match tr with
+  | []   -> ()
+  | _::tl -> slice_tr_sps_h_vals_lemma ps tl
+
+assume val slice_tr_sps_h_vals_lemma_forall:
+  unit -> Lemma (requires (True))
+               (ensures (forall ps tr. vals_trace_h (slice_tr_sps_h ps tr)))
+
+val vals_trace_h_vals_trace_lemma:
+  tr:erased trace{vals_trace_h (reveal tr)}
+  -> Lemma (requires (True)) (ensures (vals_trace tr))
+let vals_trace_h_vals_trace_lemma tr = ()
+
+val slice_tr_sps: prins -> tr:erased trace -> Tot (tr':erased trace{vals_trace tr'})
+let slice_tr_sps ps tr =
+  let tr' = elift1 (slice_tr_sps_h ps) tr in
+  slice_tr_sps_h_vals_lemma_forall ();
+  let _ = cut (b2t (reveal tr' = slice_tr_sps_h ps (reveal tr))) in
+  let _ = cut (b2t (vals_trace_h (reveal tr'))) in
+  tr'
+
 val slice_f_sps: ps:prins -> f:frame{Frame.m f = Mode Sec ps /\
                                      is_sec_frame (Frame.f f)}
                  -> Tot frame
-let slice_f_sps ps (Frame m en f') = Frame m (slice_en_sps ps en)
-                                             (slice_f'_sps ps f')
+let slice_f_sps ps (Frame m en f' tr) = Frame m (slice_en_sps ps en)
+                                                (slice_f'_sps ps f')
+				      	        (slice_tr_sps ps tr)
 
 val slice_s_sps: ps:prins -> s:stack{stack_inv s (Mode Sec ps) Source}
                  -> Tot (r:stack{stack_target_inv r (Mode Sec ps)})
@@ -142,9 +177,9 @@ let slice_t_sps ps t = match t with
   | T_val v -> T_val (D_v.v (slice_v_sps ps v))
 
 val slice_c_sps: c:sconfig{is_sec c} -> Tot tconfig
-let slice_c_sps (Conf _ (Mode Sec ps) s en t) =
+let slice_c_sps (Conf _ (Mode Sec ps) s en t tr) =
     Conf Target (Mode Sec ps) (slice_s_sps ps s) (slice_en_sps ps en)
-                (slice_t_sps ps t)
+                (slice_t_sps ps t) (slice_tr_sps ps tr)
 
 val env_upd_slice_lemma_ps: #meta:v_meta -> ps:prins -> en:env -> x:varname
                             -> v:value meta
@@ -236,6 +271,37 @@ let rec get_next_match_exp_lemma_ps #meta ps pats v = match pats with
   | []    -> ()
   | _::tl -> get_next_match_exp_lemma_ps #meta ps tl v
 
+val slice_h_append_lemma_sps:
+  ps:prins -> tr1:trace -> tr2:trace
+  -> Lemma (requires (True))
+          (ensures (slice_tr_sps_h ps (append tr1 tr2) = append (slice_tr_sps_h ps tr1) (slice_tr_sps_h ps tr2)))
+let rec slice_h_append_lemma_sps ps tr1 tr2 = match tr1 with
+  | []   -> ()
+  | _::tl -> slice_h_append_lemma_sps ps tl tr2
+
+assume val slice_h_append_lemma_forall_sps:
+  unit -> Lemma (requires (True))
+               (ensures (forall ps tr1 tr2. slice_tr_sps_h ps (append tr1 tr2) = append (slice_tr_sps_h ps tr1) (slice_tr_sps_h ps tr2)))
+
+val slice_concat_lemma_sps:
+  ps:prins -> tr1:erased trace -> tr2:erased trace
+  -> Lemma (requires (True))
+          (ensures (slice_tr_sps ps (concat_traces tr1 tr2) = concat_traces (slice_tr_sps ps tr1) (slice_tr_sps ps tr2)))
+    [SMTPat (slice_tr_sps ps (concat_traces tr1 tr2))]
+let slice_concat_lemma_sps ps tr1 tr2 =
+  slice_h_append_lemma_forall_sps ();
+  let _ = assert (slice_tr_sps_h ps (append (reveal tr1) (reveal tr2)) = append (slice_tr_sps_h ps (reveal tr1)) (slice_tr_sps_h ps (reveal tr2))) in
+  ()
+
+(* val slice_flat_lemma: *)
+(*   ps:prins -> t:trace *)
+(*   -> Lemma (requires (is_flat_trace t)) *)
+(*           (ensures (is_flat_trace (slice_tr_sps ps t))) *)
+(*     [SMTPat (is_flat_trace (slice_tr_sps ps t))] *)
+(* let rec slice_flat_lemma ps t = match t with *)
+(*   | []   -> () *)
+(*   | _::tl -> slice_flat_lemma ps tl *)
+
 opaque val sstep_sec_slice_lemma: c:sconfig{is_sec c}
                                   -> c':sconfig -> h:sstep c c'{if_exit_sec_then_to_sec h}
                                   -> Tot (cand (u:unit{Conf.m c' = Conf.m c})
@@ -262,9 +328,10 @@ let sstep_sec_slice_lemma c c' h = match h with
   | C_concatwire_e2 c c'   -> Conj () (C_concatwire_e2 (slice_c_sps c) (slice_c_sps c'))
   | C_app_e2 c c'          -> Conj () (C_app_e2 (slice_c_sps c) (slice_c_sps c'))
   | C_ffi_l c c'           ->
-    let Conf l (Mode Sec ps) ((Frame _ _ (F_ffi _ _ vs))::_) _ (T_val #meta v) = c in
+    let Conf l (Mode Sec ps) ((Frame _ _ (F_ffi _ es vs) tr)::_) _ (T_val #meta v) tr' = c in
     let _ = cut (b2t (slice_vs_sps ps ((D_v meta v)::vs) = (slice_v_sps ps v)::(slice_vs_sps ps vs))) in
     Conj () (C_ffi_l (slice_c_sps c) (slice_c_sps c'))
+
   | C_box_red c c'         -> Conj () (C_box_red (slice_c_sps c) (slice_c_sps c'))
   | C_match_red c c'       -> Conj () (C_match_red (slice_c_sps c) (slice_c_sps c'))
   | C_unbox_red c c'       -> Conj () (C_unbox_red (slice_c_sps c) (slice_c_sps c'))
@@ -276,31 +343,31 @@ let sstep_sec_slice_lemma c c' h = match h with
   | C_box_beta c c'        -> Conj () (C_box_beta (slice_c_sps c) (slice_c_sps c'))
   | C_let_beta c c'        -> Conj () (C_let_beta (slice_c_sps c) (slice_c_sps c'))
   | C_app_beta c c'        ->
-    let Conf _ (Mode Sec ps) _ _ (T_red (R_app v _)) = c in
+    let Conf _ (Mode Sec ps) _ _ (T_red (R_app v _)) _ = c in
     get_en_b_slice_lemma_ps v ps;
     Conj () (C_app_beta (slice_c_sps c) (slice_c_sps c'))
   | C_ffi_beta c c'        ->
-    let Conf _ (Mode Sec ps) _ _ (T_red (R_ffi fn vs)) = c in
+    let Conf _ (Mode Sec ps) _ _ (T_red (R_ffi fn vs)) _ = c in
     //valid_ffi_vs_slice_lemma_ps ps vs;
     exec_ffi_axiom_ps ps fn vs;
     Conj () (C_ffi_beta (slice_c_sps c) (slice_c_sps c'))
   | C_match_beta c c'      ->
-    let Conf _ (Mode Sec ps) _ _ (T_red (R_match v pats)) = c in
+    let Conf _ (Mode Sec ps) _ _ (T_red (R_match v pats)) _ = c in
     get_next_match_exp_lemma_ps ps pats v;
     Conj () (C_match_beta (slice_c_sps c) (slice_c_sps c'))
   | C_unbox_beta c c'      -> Conj () (C_unbox_beta (slice_c_sps c) (slice_c_sps c'))
   | C_mkwire_beta c c'     ->
-    let Conf _ (Mode _ ps) _ _ (T_red (R_mkwire (V_const (C_prins ps')) v)) = c in
+    let Conf _ (Mode _ ps) _ _ (T_red (R_mkwire (V_const (C_prins ps')) v)) _ = c in
     subset_intersect_lemma ps ps';
     meta_empty_can_b_same_slice v ps;
     slice_const_wire_sps_lemma ps ps' v;
     Conj () (C_mkwire_beta (slice_c_sps c) (slice_c_sps c'))
   | C_projwire_beta c c'   ->
-    let Conf _ (Mode Sec ps) _ _ (T_red (R_projwire p (V_wire eps _))) = c in
+    let Conf _ (Mode Sec ps) _ _ (T_red (R_projwire p (V_wire eps _))) _ = c in
     let _ = cut (b2t (mem p (intersect eps ps))) in
     Conj () (C_projwire_beta (slice_c_sps c) (slice_c_sps c'))
   | C_concatwire_beta c c' ->
-    let Conf _ (Mode _ ps) _ _ (T_red (R_concatwire (V_wire eps1 w1) (V_wire eps2 w2))) = c in
+    let Conf _ (Mode _ ps) _ _ (T_red (R_concatwire (V_wire eps1 w1) (V_wire eps2 w2))) _ = c in
     de_morgan_intersect_over_union eps1 eps2 ps;
     slice_wire_compose_lemma_ps #eps1 #eps2 w1 w2 ps;
     Conj () (C_concatwire_beta (slice_c_sps c) (slice_c_sps c'))
@@ -308,7 +375,7 @@ let sstep_sec_slice_lemma c c' h = match h with
   | C_assec_e c c'         -> Conj () (C_assec_e (slice_c_sps c) (slice_c_sps c'))
   | C_assec_red c c'       -> Conj () (C_assec_red (slice_c_sps c) (slice_c_sps c'))
   | C_assec_beta c c'      ->
-    let Conf _ (Mode Sec ps) _ _ (T_red (R_assec _ v)) = c in
+    let Conf _ (Mode Sec ps) _ _ (T_red (R_assec _ v)) _ = c in
     get_en_b_slice_lemma_ps v ps;
     Conj () (C_assec_beta (slice_c_sps c) (slice_c_sps c'))
   | C_assec_ret c c'       -> Conj () (C_assec_ret (slice_c_sps c) (slice_c_sps c'))
@@ -375,11 +442,22 @@ let slice_f' p f = match f with
   | F_ffi    fn es vs -> F_ffi fn es (slice_vs p vs)
   | F_match         _ -> f
 
+val slice_tr_h: prin -> trace -> Tot trace
+let rec slice_tr_h p = function
+  | []                -> []
+  | (Tr_val v)::tl       -> (Tr_val (D_v.v (slice_v p v)))::slice_tr_h p tl
+  | (Tr_scope ps tr)::tl ->
+    let tr' = if mem p ps then slice_tr_h p tr else [] in
+    append tr' (slice_tr_h p tl)
+
+val slice_tr: prin -> erased trace -> Tot (erased trace)
+let slice_tr p tr = elift1 (slice_tr_h p) tr
+
 val slice_f: p:prin -> f:frame{Mode.m (Frame.m f) = Par    /\
                                mem p (Mode.ps (Frame.m f))}
                     -> Tot frame
-let slice_f p (Frame _ en f) = Frame (Mode Par (singleton p)) (slice_en p en)
-                                     (slice_f' p f)
+let slice_f p (Frame _ en f tr) = Frame (Mode Par (singleton p)) (slice_en p en)
+                                        (slice_f' p f) (slice_tr p tr)
 
 val slice_s: p:prin -> s:stack
              -> Tot (r:stack{stack_target_inv r (Mode Par (singleton p))})
@@ -401,18 +479,18 @@ let slice_t p t = match t with
 
 val get_sec_ret_env: m:mode{Mode.m m = Sec} -> s:stack{stack_source_inv s m}
                      -> Tot env
-let rec get_sec_ret_env m (Cons (Frame m' en s) tl) =
+let rec get_sec_ret_env m (Cons (Frame m' en _ _) tl) =
   if Mode.m m' = Par then en else get_sec_ret_env m tl
 
 val slice_c: prin -> sconfig -> Tot tconfig
-let rec slice_c p (Conf Source (Mode as_m ps) s en t) =
-  let en', t' =
-    if not (mem p ps) then empty_env, T_val V_emp
+let rec slice_c p (Conf Source (Mode as_m ps) s en t tr) =
+  let en', t', tr' =
+    if not (mem p ps) then empty_env, T_val V_emp, hide []
     else
-      if as_m = Par then slice_en p en, slice_t p t
-      else slice_en p (get_sec_ret_env (Mode as_m ps) s), T_sec_wait
+      if as_m = Par then slice_en p en, slice_t p t, slice_tr p tr
+      else slice_en p (get_sec_ret_env (Mode as_m ps) s), T_sec_wait, hide []
   in
-  Conf Target (Mode Par (singleton p)) (slice_s p s) en' t'
+  Conf Target (Mode Par (singleton p)) (slice_s p s) en' t' tr'
 
 (**********)
 
@@ -720,6 +798,85 @@ let rec get_next_match_exp_lemma #meta p pats v = match pats with
   | []    -> ()
   | _::tl -> get_next_match_exp_lemma #meta p tl v
 
+val append_assoc: l1:list 'a -> l2:list 'a -> l3:list 'a ->
+  Lemma (requires True)
+        (ensures ((append l1 (append l2 l3)) = (append (append l1 l2) l3)))
+let rec append_assoc l1 l2 l3 = match l1 with
+    | [] -> ()
+    | hd::tl -> append_assoc tl l2 l3
+
+val slice_h_append_lemma:
+  p:prin -> tr1:trace -> tr2:trace
+  -> Lemma (requires (True))
+          (ensures (slice_tr_h p (append tr1 tr2) = append (slice_tr_h p tr1) (slice_tr_h p tr2)))
+let rec slice_h_append_lemma p tr1 tr2 = match tr1 with
+  | []                  -> ()
+  | (Tr_val _)::tl       -> slice_h_append_lemma p tl tr2
+  | (Tr_scope ps tr)::tl ->
+    if mem p ps then
+      let _ = slice_h_append_lemma p tl tr2 in
+      let _ = append_assoc (slice_tr_h p tr) (slice_tr_h p tl) (slice_tr_h p tr2) in
+      ()
+    else
+      slice_h_append_lemma p tl tr2
+
+assume val slice_h_append_lemma_forall:
+  unit -> Lemma (requires (True))
+               (ensures (forall p tr1 tr2. slice_tr_h p (append tr1 tr2) = append (slice_tr_h p tr1) (slice_tr_h p tr2)))
+
+val slice_concat_lemma:
+  p:prin -> tr1:erased trace -> tr2:erased trace
+  -> Lemma (requires (True))
+          (ensures (slice_tr p (concat_traces tr1 tr2) = concat_traces (slice_tr p tr1) (slice_tr p tr2)))
+    [SMTPat (slice_tr p (concat_traces tr1 tr2))]
+let slice_concat_lemma p tr1 tr2 =
+  slice_h_append_lemma_forall ();
+  let _ = assert (slice_tr_h p (append (reveal tr1) (reveal tr2)) = append (slice_tr_h p (reveal tr1)) (slice_tr_h p (reveal tr2))) in
+  ()
+
+val append_l_nil: l:list 'a ->
+  Lemma (requires True)
+        (ensures (append l [] = l))
+let rec append_l_nil = function
+  | [] -> ()
+  | hd::tl -> append_l_nil tl
+
+val scoped_trace_mem_slice_lemma_h:
+  p:prin -> ps:prins{mem p ps} -> tr:trace
+  -> Lemma (requires (True))
+          (ensures (slice_tr_h p [ Tr_scope ps tr] = slice_tr_h p tr))
+let scoped_trace_mem_slice_lemma_h p ps tr = append_l_nil (slice_tr_h p tr)
+
+assume val scoped_trace_mem_slice_lemma_forall_h:
+  unit ->
+  Lemma (requires (True))
+        (ensures (forall p ps tr. mem p ps ==> slice_tr_h p [ Tr_scope ps tr] = slice_tr_h p tr))
+
+val scoped_trace_mem_slice_lemma:
+  p:prin -> ps:prins{mem p ps} -> tr:erased trace
+  -> Lemma (requires (True))
+          (ensures (slice_tr p (hide ([ Tr_scope ps (reveal tr) ])) = slice_tr p tr))
+let scoped_trace_mem_slice_lemma p ps tr =
+  scoped_trace_mem_slice_lemma_forall_h ()
+
+val scoped_trace_not_mem_slice_lemma_h:
+  p:prin -> ps:prins{not (mem p ps)} -> tr:trace
+  -> Lemma (requires (True))
+          (ensures (slice_tr_h p [ Tr_scope ps tr ] = []))
+let scoped_trace_not_mem_slice_lemma_h p ps tr = append_l_nil []	  
+
+assume val scoped_trace_not_mem_slice_lemma_forall_h:
+  unit ->
+  Lemma (requires (True))
+        (ensures (forall p (ps:prins) tr. not (mem p ps) ==> slice_tr_h p [ Tr_scope ps tr] = []))
+
+val scoped_trace_not_mem_slice_lemma:
+  p:prin -> ps:prins{not (mem p ps)} -> tr:erased trace
+  -> Lemma (requires (True))
+          (ensures (slice_tr p (hide ([ Tr_scope ps (reveal tr) ])) = hide []))
+let scoped_trace_not_mem_slice_lemma p ps tr =
+  scoped_trace_not_mem_slice_lemma_forall_h ()
+
 opaque val sstep_par_slice_lemma: c:sconfig -> c':sconfig
                                   -> h:sstep c c'{if_enter_sec_then_from_sec h /\
                                                   if_exit_sec_then_to_sec h}
@@ -732,147 +889,147 @@ let sstep_par_slice_lemma c c' h p =
   (*if is_sec c then IntroL ()
   else*)
   match h with
-    | C_aspar_ps (Conf _ m _ _ _) _ ->
+    | C_aspar_ps (Conf _ m _ _ _ _) _ ->
       if is_sec c || not (mem p (Mode.ps m)) then IntroL ()
       else IntroR (C_aspar_ps (slice_c p c) (slice_c p c'))
-    | C_box_ps (Conf _ m _ _ _) _ ->
+    | C_box_ps (Conf _ m _ _ _ _) _ ->
       if is_sec c || not (mem p (Mode.ps m)) then IntroL ()
       else IntroR (C_box_ps (slice_c p c) (slice_c p c'))
-    | C_unbox (Conf _ m _ _ _) _ ->
+    | C_unbox (Conf _ m _ _ _ _) _ ->
       if is_sec c || not (mem p (Mode.ps m)) then IntroL ()
       else IntroR (C_unbox (slice_c p c) (slice_c p c'))
-    | C_mkwire_e1 (Conf _ m _ _ _) _ ->
+    | C_mkwire_e1 (Conf _ m _ _ _ _) _ ->
       if is_sec c || not (mem p (Mode.ps m)) then IntroL ()
       else IntroR (C_mkwire_e1 (slice_c p c) (slice_c p c'))
-    | C_projwire_p (Conf _ m _ _ _) _ ->
+    | C_projwire_p (Conf _ m _ _ _ _) _ ->
       if is_sec c || not (mem p (Mode.ps m)) then IntroL ()
       else IntroR (C_projwire_p (slice_c p c) (slice_c p c'))
-    | C_concatwire_e1 (Conf _ m _ _ _) _ ->
+    | C_concatwire_e1 (Conf _ m _ _ _ _) _ ->
       if is_sec c || not (mem p (Mode.ps m)) then IntroL ()
       else IntroR (C_concatwire_e1 (slice_c p c) (slice_c p c'))
-    | C_const (Conf _ m _ _ _) _ ->
+    | C_const (Conf _ m _ _ _ _) _ ->
       if is_sec c || not (mem p (Mode.ps m)) then IntroL ()
       else IntroR (C_const (slice_c p c) (slice_c p c'))
-    | C_var (Conf _ m _ _ _) _ ->
+    | C_var (Conf _ m _ _ _ _) _ ->
       if is_sec c || not (mem p (Mode.ps m)) then IntroL ()
       else IntroR (C_var (slice_c p c) (slice_c p c'))
-    | C_let_e1 (Conf _ m _ _ _) _ ->
+    | C_let_e1 (Conf _ m _ _ _ _) _ ->
       if is_sec c || not (mem p (Mode.ps m)) then IntroL ()
       else IntroR (C_let_e1 (slice_c p c) (slice_c p c'))
-    | C_abs (Conf _ m _ en _) _ ->
+    | C_abs (Conf _ m _ en _ _) _ ->
       if is_sec c || not (mem p (Mode.ps m)) then IntroL ()
       else
         IntroR (C_abs (slice_c p c) (slice_c p c'))
-    | C_fix (Conf _ m _ en _) _ ->
+    | C_fix (Conf _ m _ en _ _) _ ->
       if is_sec c || not (mem p (Mode.ps m)) then IntroL ()
       else
         IntroR (C_fix (slice_c p c) (slice_c p c'))
-    | C_empabs (Conf _ m _ en _) _ ->
+    | C_empabs (Conf _ m _ en _ _) _ ->
       if is_sec c || not (mem p (Mode.ps m)) then IntroL ()
       else
         IntroR (C_empabs (slice_c p c) (slice_c p c'))
-    | C_app_e1 (Conf _ m _ _ _) _ ->
+    | C_app_e1 (Conf _ m _ _ _ _) _ ->
       if is_sec c || not (mem p (Mode.ps m)) then IntroL ()
       else IntroR (C_app_e1 (slice_c p c) (slice_c p c'))
-    | C_ffi_e (Conf _ m _ _ _) _ ->
+    | C_ffi_e (Conf _ m _ _ _ _) _ ->
       if is_sec c || not (mem p (Mode.ps m)) then IntroL ()
       else IntroR (C_ffi_e (slice_c p c) (slice_c p c'))
-    | C_match_e (Conf _ m _ _ _) _ ->
+    | C_match_e (Conf _ m _ _ _ _) _ ->
       if is_sec c || not (mem p (Mode.ps m)) then IntroL ()
       else IntroR (C_match_e (slice_c p c) (slice_c p c'))
-    | C_aspar_e (Conf _ m _ _ _) _ ->
+    | C_aspar_e (Conf _ m _ _ _ _) _ ->
       if is_sec c || not (mem p (Mode.ps m)) then IntroL ()
       else IntroR (C_aspar_e (slice_c p c) (slice_c p c'))
-    | C_box_e (Conf _ m _ _ _) _ ->
+    | C_box_e (Conf _ m _ _ _ _) _ ->
       if is_sec c || not (mem p (Mode.ps m)) then IntroL ()
       else IntroR (C_box_e (slice_c p c) (slice_c p c'))
-    | C_mkwire_e2 (Conf _ m _ _ _) _ ->
+    | C_mkwire_e2 (Conf _ m _ _ _ _) _ ->
       if is_sec c || not (mem p (Mode.ps m)) then IntroL ()
       else IntroR (C_mkwire_e2 (slice_c p c) (slice_c p c'))
-    | C_projwire_e (Conf _ m _ _ _) _ ->
+    | C_projwire_e (Conf _ m _ _ _ _) _ ->
       if is_sec c || not (mem p (Mode.ps m)) then IntroL ()
       else IntroR (C_projwire_e (slice_c p c) (slice_c p c'))
-    | C_concatwire_e2 (Conf _ m _ _ _) _ ->
+    | C_concatwire_e2 (Conf _ m _ _ _ _) _ ->
       if is_sec c || not (mem p (Mode.ps m)) then IntroL ()
       else IntroR (C_concatwire_e2 (slice_c p c) (slice_c p c'))
-    | C_app_e2 (Conf _ m _ _ _) _ ->
+    | C_app_e2 (Conf _ m _ _ _ _) _ ->
       if is_sec c || not (mem p (Mode.ps m)) then IntroL ()
       else IntroR (C_app_e2 (slice_c p c) (slice_c p c'))
-    | C_ffi_l (Conf _ m _ _ _) _ ->
+    | C_ffi_l (Conf _ m _ _ _ _) _ ->
       if is_sec c || not (mem p (Mode.ps m)) then IntroL ()
       else IntroR (C_ffi_l (slice_c p c) (slice_c p c'))
-    | C_match_red (Conf _ m _ _ _) _ ->
+    | C_match_red (Conf _ m _ _ _ _) _ ->
       if is_sec c || not (mem p (Mode.ps m)) then IntroL ()
       else IntroR (C_match_red (slice_c p c) (slice_c p c'))
-    | C_aspar_red (Conf _ m _ _ _) _ ->
+    | C_aspar_red (Conf _ m _ _ _ _) _ ->
       if is_sec c || not (mem p (Mode.ps m)) then IntroL ()
       else IntroR (C_aspar_red (slice_c p c) (slice_c p c'))
-    | C_box_red (Conf _ m s _ _) _ ->
+    | C_box_red (Conf _ m s _ _ _) _ ->
       if is_sec c || not (mem p (Mode.ps m)) then IntroL ()
       else IntroR (C_box_red (slice_c p c) (slice_c p c'))
-    | C_unbox_red (Conf _ m _ _ _) _ ->
+    | C_unbox_red (Conf _ m _ _ _ _) _ ->
       if is_sec c || not (mem p (Mode.ps m)) then IntroL ()
       else IntroR (C_unbox_red (slice_c p c) (slice_c p c'))
-    | C_mkwire_red (Conf _ m _ _ _) _ ->
+    | C_mkwire_red (Conf _ m _ _ _ _) _ ->
       if is_sec c || not (mem p (Mode.ps m)) then IntroL ()
       else IntroR (C_mkwire_red (slice_c p c) (slice_c p c'))
-    | C_projwire_red (Conf _ m _ _ _) _ ->
+    | C_projwire_red (Conf _ m _ _ _ _) _ ->
       if is_sec c || not (mem p (Mode.ps m)) then IntroL ()
       else IntroR (C_projwire_red (slice_c p c) (slice_c p c'))
-    | C_concatwire_red (Conf _ m _ _ _) _ ->
+    | C_concatwire_red (Conf _ m _ _ _ _) _ ->
       if is_sec c || not (mem p (Mode.ps m)) then IntroL ()
       else IntroR (C_concatwire_red (slice_c p c) (slice_c p c'))
-    | C_let_red (Conf _ m _ _ _) _ ->
+    | C_let_red (Conf _ m _ _ _ _) _ ->
       if is_sec c || not (mem p (Mode.ps m)) then IntroL ()
       else IntroR (C_let_red (slice_c p c) (slice_c p c'))
-    | C_app_red (Conf _ m _ _ _) _ ->
+    | C_app_red (Conf _ m _ _ _ _) _ ->
       if is_sec c || not (mem p (Mode.ps m)) then IntroL ()
       else IntroR (C_app_red (slice_c p c) (slice_c p c'))
-    | C_let_beta (Conf _ m _ _ _) _ ->
+    | C_let_beta (Conf _ m _ _ _ _) _ ->
       if is_sec c || not (mem p (Mode.ps m)) then IntroL ()
       else
-        let Conf _ _ _ en (T_red (R_let x v _)) = c in
+        let Conf _ _ _ en (T_red (R_let x v _)) _ = c in
         let _ = env_upd_slice_lemma p en x v in
         IntroR (C_let_beta (slice_c p c) (slice_c p c'))
-    | C_app_beta (Conf _ m _ _ _) _ ->
+    | C_app_beta (Conf _ m _ _ _ _) _ ->
       if is_sec c || not (mem p (Mode.ps m)) then IntroL ()
       else
         let T_red (R_app f v) = Conf.t c in
         let (en, x, _) = get_en_b f in
         env_upd_slice_lemma p en x v;
         IntroR (C_app_beta (slice_c p c) (slice_c p c'))
-    | C_ffi_beta (Conf _ m _ _ _) c' ->
+    | C_ffi_beta (Conf _ m _ _ _ _) c' ->
       if is_sec c || not (mem p (Mode.ps m)) then IntroL ()
       else
-        let Conf _ _ _ _ (T_red (R_ffi fn vs)) = c in
+        let Conf _ _ _ _ (T_red (R_ffi fn vs)) _ = c in
         //valid_ffi_vs_slice_lemma p vs;
         exec_ffi_axiom p fn vs;
         IntroR (C_ffi_beta (slice_c p c) (slice_c p c'))
-    | C_match_beta (Conf _ m _ _ _) c' ->
+    | C_match_beta (Conf _ m _ _ _ _) c' ->
       if is_sec c || not (mem p (Mode.ps m)) then IntroL ()
       else
-        let Conf _ _ _ _ (T_red (R_match v pats)) = c in
+        let Conf _ _ _ _ (T_red (R_match v pats)) _ = c in
         get_next_match_exp_lemma p pats v;
         IntroR (C_match_beta (slice_c p c) (slice_c p c'))
-    | C_aspar_beta (Conf _ m _ _ _) _ ->
+    | C_aspar_beta (Conf _ m _ _ _ _) _ ->
       if is_sec c || not (mem p (Mode.ps m)) then IntroL ()
       else
         let T_red (R_aspar _ v) = Conf.t c in
         let (en, x, _) = get_en_b v in
         env_upd_slice_lemma p en x (V_const (C_unit));
         IntroR (C_aspar_beta (slice_c p c) (slice_c p c'))
-    | C_box_beta (Conf _ m _ _ (T_red (R_box ps _))) _ ->
+    | C_box_beta (Conf _ m _ _ (T_red (R_box ps _)) _) _ ->
       if is_sec c || not (mem p (Mode.ps m)) then IntroL ()
       else
         IntroR (C_box_beta (slice_c p c) (slice_c p c'))
-    | C_unbox_beta (Conf _ m _ _ _) _ ->
+    | C_unbox_beta (Conf _ m _ _ _ _) _ ->
       if is_sec c || not (mem p (Mode.ps m)) then IntroL ()
       else
         IntroR (C_unbox_beta (slice_c p c) (slice_c p c'))
-    | C_mkwire_beta (Conf _ m _ _ _) _ ->
+    | C_mkwire_beta (Conf _ m _ _ _ _) _ ->
       if is_sec c || not (mem p (Mode.ps m)) then IntroL ()
       else
-        let Conf _ (Mode Par _) _ _ (T_red (R_mkwire (V_const (C_prins ps')) (V_box ps'' v))) = c in
+        let Conf _ (Mode Par _) _ _ (T_red (R_mkwire (V_const (C_prins ps')) (V_box ps'' v))) _ = c in
         if not (mem p ps') then
           let _ =
             slice_wire_p_lemma_not_mem p ps' v;
@@ -885,37 +1042,40 @@ let sstep_par_slice_lemma c c' h p =
             mem_intersect_lemma_mem p ps'
           in
           IntroR (C_mkwire_beta (slice_c p c) (slice_c p c'))
-    | C_projwire_beta (Conf _ m _ _ _) _ ->
+    | C_projwire_beta (Conf _ m _ _ _ _) _ ->
       if is_sec c || not (mem p (Mode.ps m)) then IntroL ()
       else
         IntroR (C_projwire_beta (slice_c p c) (slice_c p c'))
-    | C_concatwire_beta (Conf _ m _ _ _) _ ->
+    | C_concatwire_beta (Conf _ m _ _ _ _) _ ->
       if is_sec c || not (mem p (Mode.ps m)) then IntroL ()
       else
-        let Conf _ _ _ _ (T_red (R_concatwire (V_wire eps1 w1) (V_wire eps2 w2))) = c in
+        let Conf _ _ _ _ (T_red (R_concatwire (V_wire eps1 w1) (V_wire eps2 w2))) _ = c in
         slice_wire_compose_lemma #eps1 #eps2 w1 w2 p;
         de_morgan_intersect_over_union eps1 eps2 (singleton p);
         IntroR (C_concatwire_beta (slice_c p c) (slice_c p c'))
-    | C_aspar_ret (Conf _ m s _ _) _ ->
-      if mem p (Mode.ps m) then
-        IntroR (C_aspar_ret (slice_c p c) (slice_c p c'))
-      else if mem p (Mode.ps (Frame.m (Cons.hd s))) then
-        IntroR (C_aspar_ret (slice_c p c) (slice_c p c'))
+    | C_aspar_ret (Conf _ m s _ _ _) _ ->
+      let Conf _ (Mode _ ps) ((Frame m' _ (F_aspar_ret ps') tr)::s) _ _ tr' = c in
+      if mem p ps then
+	let _ = scoped_trace_mem_slice_lemma p ps tr' in
+	IntroR (C_aspar_ret (slice_c p c) (slice_c p c'))
+      else if mem p (Mode.ps m') then
+	let _ = scoped_trace_not_mem_slice_lemma p ps tr' in
+	IntroR (C_aspar_ret (slice_c p c) (slice_c p c'))
       else IntroL ()
-    | C_assec_ps (Conf _ m _ _ _) _ ->
+    | C_assec_ps (Conf _ m _ _ _ _) _ ->
       if is_sec c || not (mem p (Mode.ps m)) then IntroL ()
       else
         IntroR (C_assec_ps (slice_c p c) (slice_c p c'))
-    | C_assec_e (Conf _ m _ _ _) _ ->
+    | C_assec_e (Conf _ m _ _ _ _) _ ->
       if is_sec c || not (mem p (Mode.ps m)) then IntroL ()
       else
         IntroR (C_assec_e (slice_c p c) (slice_c p c'))
-    | C_assec_red (Conf _ m _ _ _) _ ->
+    | C_assec_red (Conf _ m _ _ _ _) _ ->
       if is_sec c || not (mem p (Mode.ps m)) then IntroL ()
       else
         IntroR (C_assec_red (slice_c p c) (slice_c p c'))
     | C_assec_beta _ _ -> IntroL ()
-    | C_assec_ret (Conf _ m _ _ _) _ -> IntroL ()
+    | C_assec_ret _ _ -> IntroL ()
 
 #reset-options
 (**********)
@@ -962,7 +1122,7 @@ opaque val get_env_m:
 let rec get_env_m #ps' pi ps =
   let Some p = choose ps in
   let ps_rest = remove p ps in
-  let Some (Conf _ _ _ _ (T_red (R_assec _ v))) = select p (fst pi) in
+  let Some (Conf _ _ _ _ (T_red (R_assec _ v)) _) = select p (fst pi) in
   let (en, _, _) = get_en_b v in
   if ps_rest = empty then update p en mempty
   else
@@ -971,8 +1131,8 @@ let rec get_env_m #ps' pi ps =
 
 val step_p_to_wait: c:tconfig -> p:prin -> Tot tconfig
 let step_p_to_wait c p =
-  let Conf l m s en _ = c in
-  Conf l m ((Frame m en F_assec_ret)::s) en T_sec_wait
+  let Conf l m s en _ tr = c in
+  Conf l m ((Frame m en F_assec_ret tr)::s) en T_sec_wait (hide [])
 
 opaque val step_ps_to_wait:
   #ps':prins -> pi:tpar ps' -> ps:prins{forall p. mem p ps ==> contains p pi}
@@ -996,7 +1156,7 @@ val tstep_assec:
   -> Tot (protocol ps')
 let tstep_assec #ps' pi ps x e =
   let env = update_env (compose_envs_m ps (get_env_m pi ps)) x (V_const C_unit) in
-  let tsec = Conf Target (Mode Sec ps) [] env (T_exp e) in
+  let tsec = Conf Target (Mode Sec ps) [] env (T_exp e) (hide []) in
   (step_ps_to_wait #ps' (fst pi) ps, update ps tsec (snd pi))
 
 type waiting_config (c:tconfig) =
@@ -1012,15 +1172,16 @@ type tpre_assec_ret (#ps':prins) (pi:protocol ps') (ps:prins) =
   is_value (Some.v (select ps (snd pi))) /\ (Conf.s (Some.v (select ps (snd pi))) = []) /\
   ps_sec_waiting pi ps
 
-val ret_sec_value_to_p: sec_c:tconfig{is_value sec_c} -> c:tconfig{waiting_config c}
+val ret_sec_value_to_p: sec_c:tconfig{is_sec sec_c /\ is_value sec_c} -> c:tconfig{waiting_config c}
                         -> p:prin -> Tot tconfig
 let ret_sec_value_to_p sec_c c p =
-  let Conf l _ ((Frame m en F_assec_ret)::s) _ _ = c in
+  let Conf l _ ((Frame m en F_assec_ret tr)::s) _ _ _ = c in
   let D_v _ v = c_value sec_c in
-  Conf l m s en (T_val (D_v.v (slice_v p v)))
+  let D_v _ v' = slice_v p v in
+  Conf l m s en (T_val v') (concat_traces tr (hide [ Tr_val v' ]))
 
 opaque val ret_sec_value_to_ps:
-  #ps':prins -> pi:tpar ps' -> sec_c:tconfig{is_value sec_c}
+  #ps':prins -> pi:tpar ps' -> sec_c:tconfig{is_sec sec_c /\ is_value sec_c}
   -> ps:prins{forall p. mem p ps ==> (contains p pi /\ waiting_config (Some.v (select p pi)))}
   -> Tot (pi':tpar ps'{forall p. (mem p ps ==>
                                   select p pi' =
@@ -1638,7 +1799,7 @@ opaque val sstep_par_to_sec_en_compose_lemma:
                                select p (get_env_m #ps (slice_c_ps ps c) (Mode.ps (Conf.m c))) =
                                Some (slice_en p (MkTuple3._1 (get_en_b (R_assec.v (T_red.r (Conf.t c))))))))
 let sstep_par_to_sec_en_compose_lemma #c #c' h ps =
-  let Conf _ _ _ _ (T_red (R_assec _ v)) = c in
+  let Conf _ _ _ _ (T_red (R_assec _ v)) _ = c in
   slice_clos_lem v
 
 opaque val forward_simulation_enter_sec:
@@ -1646,7 +1807,7 @@ opaque val forward_simulation_enter_sec:
   -> ps:prins{subset (Mode.ps (Conf.m c)) ps}
   -> Tot (pstep #ps (slice_c_ps ps c) (slice_c_ps ps c'))
 let forward_simulation_enter_sec #c #c' h ps =
-  let Conf Source (Mode Par ps') s en (T_red (R_assec _ v)) = c in
+  let Conf Source (Mode Par ps') s en (T_red (R_assec _ v)) _ = c in
   let (en1, x, e) = get_en_b v in
 
   let pi, s = slice_c_ps ps c in
@@ -1664,8 +1825,8 @@ let forward_simulation_enter_sec #c #c' h ps =
   sstep_par_to_sec_slice_par #c #c' h ps x e;
   let _ = cut (b2t (pi_s = pi')) in
 
-  let Some (Conf _ _ st_s en_s t_s) = select ps' s_s in
-  let Some (Conf _ _ st' en' t') = select ps' s' in
+  let Some (Conf _ _ st_s en_s t_s _) = select ps' s_s in
+  let Some (Conf _ _ st' en' t' _) = select ps' s' in
 
   let _ = cut (b2t (st_s = [])) in
   let _ = cut (b2t (st' = [])) in
@@ -1851,7 +2012,7 @@ let pstep_ppar_psec_enter_confluence #ps pi pi1 pi2 h1 h2 =
   ExIntro #(protocol ps) #(fun pi3 -> cand (pstep #ps pi1 pi3) (pstep #ps pi2 pi3)) (pi3_m, s3) (Conj h13 h23)
 
 val ret_sec_value_to_ps_update_lemma:
-  ps':prins -> pi:tpar ps' -> sec_c:tconfig{is_value sec_c} -> ps:prins{forall p. mem p ps ==> (contains p pi /\ waiting_config (Some.v (select p pi)))}
+  ps':prins -> pi:tpar ps' -> sec_c:tconfig{is_sec sec_c /\ is_value sec_c} -> ps:prins{forall p. mem p ps ==> (contains p pi /\ waiting_config (Some.v (select p pi)))}
   -> p:prin{not (mem p ps) /\ mem p ps'} -> c:tconfig_par
   -> Lemma (requires (True))
            (ensures (update p c (ret_sec_value_to_ps #ps' pi sec_c ps) = ret_sec_value_to_ps #ps' (update p c pi) sec_c ps))
@@ -2015,12 +2176,12 @@ let pstep_psec_enter_psec_enter_confluence #ps pi pi1 pi2 h1 h2 =
     
     let env23 = update_env (compose_envs_m (P_sec_enter.ps h1) (get_env_m pi2 (P_sec_enter.ps h1)))
                 (P_sec_enter.x h1) (V_const C_unit) in
-    let tsec23 = Conf Target (Mode Sec (P_sec_enter.ps h1)) [] env23 (T_exp (P_sec_enter.e h1)) in
+    let tsec23 = Conf Target (Mode Sec (P_sec_enter.ps h1)) [] env23 (T_exp (P_sec_enter.e h1)) (hide []) in
     let s23 = update (P_sec_enter.ps h1) tsec23 s2 in
     
     let env13 = update_env (compose_envs_m (P_sec_enter.ps h2) (get_env_m pi1 (P_sec_enter.ps h2)))
                 (P_sec_enter.x h2) (V_const C_unit) in
-    let tsec13 = Conf Target (Mode Sec (P_sec_enter.ps h2)) [] env13 (T_exp (P_sec_enter.e h2)) in
+    let tsec13 = Conf Target (Mode Sec (P_sec_enter.ps h2)) [] env13 (T_exp (P_sec_enter.e h2)) (hide []) in
     
     let s13 = update (P_sec_enter.ps h2) tsec13 s1 in
     let _ = cut (b2t (s13 = s23)) in
@@ -2046,7 +2207,7 @@ let pstep_psec_enter_psec_exit_confluence #ps pi pi1 pi2 h1 h2 =
 
   let env' = update_env (compose_envs_m (P_sec_enter.ps h1) (get_env_m pi (P_sec_enter.ps h1)))
              (P_sec_enter.x h1) (V_const C_unit) in
-  let tsec' = Conf Target (Mode Sec (P_sec_enter.ps h1)) [] env' (T_exp (P_sec_enter.e h1)) in
+  let tsec' = Conf Target (Mode Sec (P_sec_enter.ps h1)) [] env' (T_exp (P_sec_enter.e h1)) (hide []) in
   let _ = assert (s1 = update (P_sec_enter.ps h1) tsec' s) in
   
   OrdMap.sel_upd2 (P_sec_enter.ps h1) tsec' (P_sec_exit.ps h2) s;
@@ -2065,7 +2226,7 @@ let pstep_psec_enter_psec_exit_confluence #ps pi pi1 pi2 h1 h2 =
   
   let env23 = update_env (compose_envs_m (P_sec_enter.ps h1) (get_env_m pi2 (P_sec_enter.ps h1)))
               (P_sec_enter.x h1) (V_const C_unit) in
-  let tsec23 = Conf Target (Mode Sec (P_sec_enter.ps h1)) [] env23 (T_exp (P_sec_enter.e h1)) in
+  let tsec23 = Conf Target (Mode Sec (P_sec_enter.ps h1)) [] env23 (T_exp (P_sec_enter.e h1)) (hide []) in
   let s23 = update (P_sec_enter.ps h1) tsec23 s2 in
   //let _ = cut (b2t (tsec23 = tsec')) in
 
