examples/wysteria/tinterpreter.fst
@@ -1,9 +1,11 @@
 (*--build-config
     options:--admit_fsi FStar.OrdSet --admit_fsi FStar.OrdMap --admit_fsi FStar.Set --admit_fsi Prins --admit_fsi FFI --admit_fsi Runtime;
-    other-files:ordset.fsi ordmap.fsi classical.fst set.fsi heap.fst st.fst all.fst prins.fsi ast.fst ffi.fsi sem.fst sinterpreter.fst runtime.fsi
+    other-files:ghost.fst listTot.fst ordset.fsi ordmap.fsi classical.fst set.fsi heap.fst st.fst all.fst prins.fsi ast.fst ffi.fsi sem.fst sinterpreter.fst runtime.fsi
  --*)
 
 module TargetInterpreter
+
+open FStar.Ghost
 
 open Prins
 open AST
@@ -17,10 +19,10 @@ let do_sec_comp p r =
   
 val tstep: config -> ML (option config)
 let tstep c =
-  let Conf l m s en t = c in
+  let Conf l m s en t _ = c in
   if is_T_red t && is_R_assec (T_red.r t) then
     let dv = do_sec_comp (Some.v (OrdSet.choose (Mode.ps m))) (T_red.r t) in
-    Some (Conf l m s en (T_val #(D_v.meta dv) (D_v.v dv)))
+    Some (Conf l m s en (T_val #(D_v.meta dv) (D_v.v dv)) (hide []))
   else SourceInterpreter.step c
 
 val tstep_star: config -> ML (option config)
